added filed from hk/dev/generalfixcpo

SPF.thy
@@ -8,7 +8,7 @@
 *)
 
 theory SPF
-imports SB
+imports SB CPOFix
 
 begin
   
@@ -280,6 +280,19 @@ subsection \<open>spfRestrict\<close>
   
 definition spfRestrict :: "channel set \<Rightarrow> channel set \<Rightarrow> 'm SPF \<rightarrow> 'm SPF" where
 "spfRestrict In Out \<equiv> (\<Lambda> f. if (spfDom\<cdot>f = In \<and> spfRan\<cdot>f = Out) then f else (spfLeast In Out))"
+
+subsection \<open>spfFix\<close>
+
+definition spfFix ::"channel set \<Rightarrow> channel set \<Rightarrow>('m SPF \<rightarrow> 'm SPF) \<rightarrow> 'm SPF" where
+"spfFix In Out \<equiv> (\<Lambda> F.  if (spfDom\<cdot>(F\<cdot>(spfLeast In Out)) = In \<and> spfRan\<cdot>(F\<cdot>(spfLeast In Out)) = Out) then fixg (spfLeast In Out) F else (spfLeast In Out))"
+
+subsection \<open>spfStateFix\<close>
+  
+definition spfStateLeast :: "channel set \<Rightarrow> channel set \<Rightarrow>('s1 \<Rightarrow> 'm SPF)" where
+"spfStateLeast In Out \<equiv> (\<lambda> x. spfLeast In Out)"
+
+definition spfStateFix ::"channel set \<Rightarrow> channel set \<Rightarrow>(('s1 \<Rightarrow>'m SPF) \<rightarrow> ('s1 \<Rightarrow>'m SPF)) \<rightarrow> ('s1 \<Rightarrow> 'm SPF)" where
+"spfStateFix In Out \<equiv> (\<Lambda> F.  if \<forall>x. (spfDom\<cdot>((F\<cdot>(spfStateLeast In Out)) x) = In \<and> spfRan\<cdot>((F\<cdot>(spfStateLeast In Out)) x) = Out) then fixg (spfStateLeast In Out) F else (spfStateLeast In Out))"  
 
 (* ----------------------------------------------------------------------- *)
   section \<open>Lemmas on 'm SPF's\<close>
@@ -1349,10 +1362,249 @@ next
     by (simp add: spfLeast_ran spfRestrict_cont spfRestrict_def)
 qed 
     
+subsection \<open>spfFix\<close>      
+  
+lemma spfFix_mono[simp]: "monofun (\<lambda> F.  if (spfDom\<cdot>(F\<cdot>(spfLeast In Out)) = In \<and> spfRan\<cdot>(F\<cdot>(spfLeast In Out)) = Out) then fixg (spfLeast In Out) F else (spfLeast In Out))"
+proof(rule monofunI)
+  fix x::"'m SPF \<rightarrow> 'm SPF" and y::"'m SPF \<rightarrow> 'm SPF"
+  assume a1:"x \<sqsubseteq> y"
+  show "(if spfDom\<cdot>(x\<cdot>(spfLeast In Out)) = In \<and> spfRan\<cdot>(x\<cdot>(spfLeast In Out)) = Out then fixg (spfLeast In Out) x else spfLeast In Out) \<sqsubseteq>
+           (if spfDom\<cdot>(y\<cdot>(spfLeast In Out)) = In \<and> spfRan\<cdot>(y\<cdot>(spfLeast In Out)) = Out then fixg (spfLeast In Out) y else spfLeast In Out)"
+  proof(cases "spfDom\<cdot>(x\<cdot>(spfLeast In Out)) = In \<and> spfRan\<cdot>(x\<cdot>(spfLeast In Out)) = Out")
+    case True
+    then  have h1:"spfDom\<cdot>(y\<cdot>(spfLeast In Out)) = In \<and> spfRan\<cdot>(y\<cdot>(spfLeast In Out)) = Out"
+      by (metis cfun_below_iff a1 spfdom_eq spfran_eq)
+    then have "fixg (spfLeast In Out) x \<sqsubseteq> fixg (spfLeast In Out) y"
+      by(simp add: fixg_def lub_iter_fixg_mono_req a1 True)
+    then show ?thesis
+      by (simp add: True h1)
+  next
+    case False
+    then show ?thesis
+      apply simp
+      using a1 cfun_below_iff spfdom_eq spfran_eq by blast
+  qed
+qed
+  
+lemma spfFix_cont[simp]: "cont (\<lambda> F.  if (spfDom\<cdot>(F\<cdot>(spfLeast In Out)) = In \<and> spfRan\<cdot>(F\<cdot>(spfLeast In Out)) = Out) then fixg (spfLeast In Out) F else (spfLeast In Out))"
+proof(rule Cont.contI2,simp)
+  fix Y:: "nat \<Rightarrow> ('m SPF \<rightarrow> 'm SPF)"
+  assume a1:"chain Y"
+  assume a2:"chain (\<lambda>i. if spfDom\<cdot>(Y i\<cdot>(spfLeast In Out)) = In \<and> spfRan\<cdot>(Y i\<cdot>(spfLeast In Out)) = Out then fixg (spfLeast In Out) (Y i) else spfLeast In Out)"
+  show "(if spfDom\<cdot>((\<Squnion>i. Y i)\<cdot>(spfLeast In Out)) = In \<and> spfRan\<cdot>((\<Squnion>i. Y i)\<cdot>(spfLeast In Out)) = Out then fixg (spfLeast In Out) (\<Squnion>i. Y i) else spfLeast In Out) \<sqsubseteq>
+         (\<Squnion>i. if spfDom\<cdot>(Y i\<cdot>(spfLeast In Out)) = In \<and> spfRan\<cdot>(Y i\<cdot>(spfLeast In Out)) = Out then fixg (spfLeast In Out) (Y i) else spfLeast In Out)"
+  proof(cases "spfDom\<cdot>((\<Squnion>i. Y i)\<cdot>(spfLeast In Out)) = In \<and> spfRan\<cdot>((\<Squnion>i. Y i)\<cdot>(spfLeast In Out)) = Out")
+    case True
+      have "\<forall>i. Y i \<sqsubseteq> Y (Suc i)"
+        by (simp add: a1 po_class.chainE)
+      then have h1:"\<forall>i. spfDom\<cdot>((Y i)\<cdot>(spfLeast In Out)) = In \<and> spfRan\<cdot>(Y i\<cdot>(spfLeast In Out)) = Out"
+        using True a1 cfun_below_iff is_ub_thelub spfdom_eq spfran_eq by blast
+    then show ?thesis
+      by(simp add: True h1 fixg_def chain_lub_lub_iter_fixg a1)
+  next
+    case False
+    then show ?thesis
+    proof -
+      have f1: "spfDom\<cdot>(Y elem_6\<cdot>(spfLeast In Out)) = spfDom\<cdot>(Lub Y\<cdot>(spfLeast In Out))"
+        by (meson a1 below_lub cfun_below_iff po_class.chain_def spfdom_eq)
+      have f2: "(if spfDom\<cdot>(Y elem_6\<cdot>(spfLeast In Out)) = In \<and> spfRan\<cdot>(Y elem_6\<cdot>(spfLeast In Out)) = Out then fixg (spfLeast In Out) (Y elem_6) else spfLeast In Out) \<sqsubseteq> (\<Squnion>n. if spfDom\<cdot>(Y n\<cdot>(spfLeast In Out)) = In \<and> spfRan\<cdot>(Y n\<cdot>(spfLeast In Out)) = Out then fixg (spfLeast In Out) (Y n) else spfLeast In Out)"
+        using a2 below_lub by blast
+      have "spfRan\<cdot>(Y elem_6\<cdot>(spfLeast In Out)) = spfRan\<cdot>(Lub Y\<cdot>(spfLeast In Out))"
+        by (meson a1 below_lub cfun_below_iff po_class.chain_def spfran_eq)
+    then show ?thesis
+      using f2 f1 False by presburger
+    qed
+  qed 
+qed
+
+
+lemma spfFix_apply[simp]: assumes "spfDom\<cdot>(F\<cdot>(spfLeast In Out)) = In" and "spfRan\<cdot>(F\<cdot>(spfLeast In Out)) = Out" 
+                          shows "spfFix In Out\<cdot>F = fixg (spfLeast In Out) F"
+  by(simp add: spfFix_def assms)
+    
+(*least Fixpoint*)
+    
+lemma spfFix_fix: assumes "spfDom\<cdot>(F\<cdot>(spfLeast In Out)) = In" and "spfRan\<cdot>(F\<cdot>(spfLeast In Out)) = Out" 
+                  shows "spfFix In Out\<cdot>F = F\<cdot>(spfFix In Out\<cdot>F)"
+proof(simp add: assms,rule fixg_fix, simp add: assms)
+  show "\<forall>y. y \<sqsubseteq> spfLeast In Out \<longrightarrow> spfLeast In Out = y"
+    by (simp add: assms fixg_fix po_eq_conv spfdom_eq spfran_eq)
+qed
+  
+lemma spfFix_least_fix: assumes "spfDom\<cdot>(F\<cdot>(spfLeast In Out)) = In" 
+                        and "spfRan\<cdot>(F\<cdot>(spfLeast In Out)) = Out" 
+                        and "F\<cdot>y = y" and "spfDom\<cdot>y = In" and "spfRan\<cdot>y = Out"
+                        shows "spfFix In Out\<cdot>F \<sqsubseteq> y"
+proof(simp add: assms, rule fixg_least_fix, simp_all add: assms)
+  show "\<forall>y. y \<sqsubseteq> spfLeast In Out \<longrightarrow> spfLeast In Out = y"
+    by (simp add: assms fixg_fix po_eq_conv spfdom_eq spfran_eq)
+qed
+
+  
+(*Test spfFix with id*)
+lemma "spfFix {c1} {c2}\<cdot>(\<Lambda> f. f) = spfLeast {c1} {c2}"
+  proof(subst spfFix_apply,simp,simp)
+    have "(\<Lambda> f. f)\<cdot>(spfLeast {c1} {c2}) = spfLeast {c1} {c2}"
+      by simp
+    then show "fixg (spfLeast {c1} {c2}) (\<Lambda> f. f) = spfLeast {c1} {c2}"
+      by (metis (mono_tags, lifting)  po_eq_conv spfFix_apply spfFix_least_fix spfLeast_bottom spfLeast_dom spfLeast_ran spfdom_eq spfran_eq)
+  qed
     
     
+subsection \<open>spfStateLeast\<close>
+        
+lemma spfStateLeast_mono: "monofun (\<lambda>x. spfLeast In Out)" 
+  by (simp add: monofunI)   
+  
+lemma spfStateLeast_cont: "cont (\<lambda>x. spfLeast In Out)"
+  by simp
+
+lemma spfStateLeast_dom [simp]: "\<forall>x. spfDom\<cdot>(spfStateLeast In Out x) = In"
+  by (metis (mono_tags, lifting) spfLeast_dom spfStateLeast_def)
+
+lemma spfStateLeast_ran[simp]: "\<forall>x. spfRan\<cdot>(spfStateLeast In Out x) = Out"
+proof - 
+  have "sbDom\<cdot>(sbLeast Out) = Out"
+    by simp
+  thus ?thesis
+    by(simp add: spfStateLeast_def)
+qed
+
+lemma spfStateLeast_apply[simp]: 
+  assumes "sbDom\<cdot>sb = In"
+  shows "\<forall>x. spfStateLeast In Out x \<rightleftharpoons> sb = sbLeast Out"
+  by(simp add: spfStateLeast_def assms)
+
+lemma spfStateLeast_bottom [simp]: assumes "\<forall>x. spfDom\<cdot>(f x) = In" and " \<forall>x. spfRan\<cdot>(f x) = Out"
+  shows "(spfStateLeast In Out) \<sqsubseteq> f"
+proof -
+  have f1: "\<forall>x. (spfStateLeast In Out x) \<sqsubseteq> f x"
+    by (simp add: assms(1) assms(2) spfStateLeast_def)
+  show ?thesis
+    by(simp add: below_fun_def f1)
+qed  
+
+subsection \<open>spfStateFix\<close>  
+
+lemma spfStateFix_mono[simp]: "monofun (\<lambda> F.  if \<forall>x. (spfDom\<cdot>((F\<cdot>(spfStateLeast In Out)) x) = In \<and> spfRan\<cdot>((F\<cdot>(spfStateLeast In Out)) x) = Out) then fixg (spfStateLeast In Out) F else (spfStateLeast In Out))"
+proof(rule monofunI)
+  fix x::"('s1 \<Rightarrow> 'm SPF) \<rightarrow> ('s1 \<Rightarrow> 'm SPF)" and y::"('s1 \<Rightarrow>'m SPF) \<rightarrow> ('s1 \<Rightarrow>'m SPF)"
+  assume a1:"x \<sqsubseteq> y"
+  show "(if \<forall>xa. spfDom\<cdot>((x\<cdot>(spfStateLeast In Out)) xa) = In \<and> spfRan\<cdot>((x\<cdot>(spfStateLeast In Out)) xa) = Out then fixg (spfStateLeast In Out) x else spfStateLeast In Out) \<sqsubseteq>
+           (if \<forall>x. spfDom\<cdot>((y\<cdot>(spfStateLeast In Out)) x) = In \<and> spfRan\<cdot>((y\<cdot>(spfStateLeast In Out)) x) = Out then fixg (spfStateLeast In Out) y else spfStateLeast In Out)"
+  proof(cases "\<forall>xa. spfDom\<cdot>((x\<cdot>(spfStateLeast In Out)) xa) = In \<and> spfRan\<cdot>((x\<cdot>(spfStateLeast In Out)) xa) = Out")
+    case True
+    then  have h1:"\<forall>xa. spfDom\<cdot>((y\<cdot>(spfStateLeast In Out)) xa) = In \<and> spfRan\<cdot>((y\<cdot>(spfStateLeast In Out)) xa) = Out"
+      by (metis (mono_tags, lifting) a1 below_fun_def cfun_below_iff spfdom_eq spfran_eq)
+    then have "fixg (spfStateLeast In Out) x \<sqsubseteq> fixg (spfStateLeast In Out) y"
+      by(simp add: fixg_def lub_iter_fixg_mono_req a1 True)
+    then show ?thesis
+      by (simp add: True h1)
+  next
+    case False
+    then have h2: "\<not> (\<forall>xa. spfDom\<cdot>((y\<cdot>(spfStateLeast In Out)) xa) = In \<and> spfRan\<cdot>((y\<cdot>(spfStateLeast In Out)) xa) = Out)"
+      by (metis (mono_tags, lifting) a1 below_fun_def cfun_below_iff spfdom_eq spfran_eq)
+    then show ?thesis
+      by (simp add: h2 False)
+  qed
+qed
+  
+lemma spfStateFix_cont[simp]: "cont (\<lambda> F.  if \<forall>x. (spfDom\<cdot>((F\<cdot>(spfStateLeast In Out)) x) = In \<and> spfRan\<cdot>((F\<cdot>(spfStateLeast In Out)) x) = Out) then fixg (spfStateLeast In Out) F else (spfStateLeast In Out))"
+proof(rule Cont.contI2,simp)
+  fix Y:: "nat \<Rightarrow> (('s1 \<Rightarrow>'m SPF) \<rightarrow> ('s1 \<Rightarrow>'m SPF))"
+  assume a1:"chain Y"
+  assume a2:"chain (\<lambda>i. if \<forall>x. spfDom\<cdot>((Y i\<cdot>(spfStateLeast In Out)) x) = In \<and> spfRan\<cdot>((Y i\<cdot>(spfStateLeast In Out)) x) = Out then fixg (spfStateLeast In Out) (Y i)
+                    else spfStateLeast In Out)"
+  show "(if \<forall>x. spfDom\<cdot>(((\<Squnion>i. Y i)\<cdot>(spfStateLeast In Out)) x) = In \<and> spfRan\<cdot>(((\<Squnion>i. Y i)\<cdot>(spfStateLeast In Out)) x) = Out then fixg (spfStateLeast In Out) (\<Squnion>i. Y i)
+          else spfStateLeast In Out) \<sqsubseteq>
+         (\<Squnion>i. if \<forall>x. spfDom\<cdot>((Y i\<cdot>(spfStateLeast In Out)) x) = In \<and> spfRan\<cdot>((Y i\<cdot>(spfStateLeast In Out)) x) = Out then fixg (spfStateLeast In Out) (Y i) else spfStateLeast In Out)"
+  proof(cases "\<forall>x. spfDom\<cdot>(((\<Squnion>i. Y i)\<cdot>(spfStateLeast In Out)) x) = In \<and> spfRan\<cdot>(((\<Squnion>i. Y i)\<cdot>(spfStateLeast In Out)) x) = Out")
+    case True
+      have "\<forall>i. Y i \<sqsubseteq> Y (Suc i)"
+        by (simp add: a1 po_class.chainE)
+      have f0:"\<forall>x. chain (\<lambda>i. (Y i\<cdot>(spfStateLeast In Out)) x)"
+        using a1 ch2ch_Rep_cfunL ch2ch_fun by fastforce    
+      then have h1:"\<forall>x i. spfDom\<cdot>((Y i\<cdot>(spfStateLeast In Out)) x) = In \<and> spfRan\<cdot>((Y i\<cdot>(spfStateLeast In Out)) x) = Out"
+        by (smt True a1 cfun_below_iff fun_below_iff is_ub_thelub spfdom_eq spfran_eq)
+    then show ?thesis
+      by(simp add: True h1 fixg_def chain_lub_lub_iter_fixg a1)
+  next
+    case False
+    have f0:"\<forall>x. chain (\<lambda>i. (Y i\<cdot>(spfStateLeast In Out)) x)"
+      using a1 ch2ch_Rep_cfunL ch2ch_fun by fastforce          
+    then have f1: "\<forall>x. spfDom\<cdot>((Y elem_6\<cdot>(spfStateLeast In Out)) x) = spfDom\<cdot>((\<Squnion>i. (Y i \<cdot>(spfStateLeast In Out)))x)"
+      proof -
+        have "chain (\<lambda>n. Y n\<cdot>(spfStateLeast In Out))"
+          by (metis a1 ch2ch_Rep_cfunL)
+        then show ?thesis
+          using f0 lub_fun spfdom_eq_lub by fastforce
+      qed
+    have f2:"\<forall>x. spfRan\<cdot>((Y elem_6\<cdot>(spfStateLeast In Out)) x) = spfRan\<cdot>((\<Squnion>i. Y i\<cdot>(spfStateLeast In Out)) x)"
+      proof -
+        have "\<And>f n s. \<not> chain f \<or> spfRan\<cdot>(f n (s::'s1)::'m SPF) = spfRan\<cdot>(Lub f s)"
+          by (metis (full_types) ch2ch_fun lub_fun spfran_eq_lub)
+        then show ?thesis
+          using a1 ch2ch_Rep_cfunL by blast
+      qed
+    have f3:"\<forall>i. \<not>(\<forall>x. spfDom\<cdot>((Y i\<cdot>(spfStateLeast In Out)) x) = In \<and> spfRan\<cdot>((Y i\<cdot>(spfStateLeast In Out)) x) = Out)"
+      using False spfdom_eq_lub spfdom_eq spfran_eq_lub spfran_eq a1 a2
+    proof -
+      { fix nn :: nat
+        have ff1: "\<And>f fa s. f \<notsqsubseteq> fa \<or> spfRan\<cdot>(f (s::'s1)::'m SPF) = spfRan\<cdot>(fa s)"
+          by (meson fun_below_iff spfran_eq)
+        have ff2: "\<And>f fa s. f \<notsqsubseteq> fa \<or> spfDom\<cdot>(f (s::'s1)::'m SPF) = spfDom\<cdot>(fa s)"
+          by (metis fun_below_iff spfdom_eq)
+        have "\<And>f n fa. \<not> chain f \<or> (f n\<cdot> (fa::'s1 \<Rightarrow> 'm SPF)::'s1 \<Rightarrow> 'm SPF) \<sqsubseteq> Lub f\<cdot>fa"
+          by (metis ch2ch_Rep_cfunL contlub_cfun_fun is_ub_thelub)
+        then have "\<exists>s sa. spfDom\<cdot>((Y nn\<cdot>(spfStateLeast In Out)) s) \<noteq> In \<or> spfRan\<cdot>((Y nn\<cdot>(spfStateLeast In Out)) sa) \<noteq> Out"
+          using ff2 ff1 False a1 by blast }
+      then show ?thesis
+        by meson
+    qed
+    have f4: "\<And>s n. spfRan\<cdot>(\<Squnion>n. (Y n\<cdot>(spfStateLeast In Out)) s) = spfRan\<cdot>((Y n\<cdot>(spfStateLeast In Out)) s)"
+        using f0 spfran_eq_lub by blast
+      have f5: "\<And>s n. spfDom\<cdot>(\<Squnion>n. (Y n\<cdot>(spfStateLeast In Out)) s) = spfDom\<cdot>((Y n\<cdot>(spfStateLeast In Out)) s)"
+        using f0 spfdom_eq_lub by blast
+    show ?thesis
+      by(simp add: f3 False)
+    qed 
+qed
+
+
+lemma spfStateFix_apply[simp]: assumes "\<forall>x. spfDom\<cdot>((F\<cdot>(spfStateLeast In Out)) x) = In" and "\<forall>x. spfRan\<cdot>((F\<cdot>(spfStateLeast In Out))x) = Out" shows "spfStateFix In Out\<cdot>F = fixg (spfStateLeast In Out) F"
+  by(simp add: spfStateFix_def assms)
     
+(*least Fixpoint*)
     
+lemma spfStateFix_fix: assumes "\<forall>x. spfDom\<cdot>((F\<cdot>(spfStateLeast In Out)) x) = In" and "\<forall>x. spfRan\<cdot>((F\<cdot>(spfStateLeast In Out))x) = Out" shows "spfStateFix In Out\<cdot>F = F\<cdot>(spfStateFix In Out\<cdot>F)"
+proof(simp add: assms,rule fixg_fix, simp add: assms)
+  show "\<forall>y. y \<sqsubseteq> spfStateLeast In Out \<longrightarrow> spfStateLeast In Out = y"
+    by (smt below_antisym below_fun_def spfLeast_bottom spfStateLeast_def spfStateLeast_dom spfStateLeast_ran spfdom_eq spfran_eq)
+qed
+  
+lemma spfStateFix_least_fix: assumes "\<forall>x. spfDom\<cdot>((F\<cdot>(spfStateLeast In Out)) x) = In" 
+                             and "\<forall>x. spfRan\<cdot>((F\<cdot>(spfStateLeast In Out))x) = Out" 
+                             and "F\<cdot>y = y" and "\<forall>x. spfDom\<cdot>(y x) = In" and "\<forall>x. spfRan\<cdot>(y x) = Out"
+                           shows "spfStateFix In Out\<cdot>F \<sqsubseteq> y"
+proof(simp add: assms, rule fixg_least_fix, simp_all add: assms)
+  show "\<forall>y. y \<sqsubseteq> spfStateLeast In Out \<longrightarrow> spfStateLeast In Out = y"
+    by (smt below_antisym below_fun_def spfLeast_bottom spfStateLeast_def spfStateLeast_dom spfStateLeast_ran spfdom_eq spfran_eq)
+qed
+
+(*Test spfStateFix with id*)
+
+lemma "spfStateFix {c1} {c2}\<cdot>(\<Lambda> f. f) = spfStateLeast {c1} {c2}"
+proof(subst spfStateFix_apply,simp,simp)
+  have f1:"(\<Lambda> f. f)\<cdot>(spfStateLeast {c1} {c2}) = spfStateLeast {c1} {c2}"
+    by(simp)
+  then have f2:"fixg (spfStateLeast {c1} {c2}) (\<Lambda> f. f) \<sqsubseteq> spfStateLeast {c1} {c2}"
+    by (metis spfStateFix_apply spfStateFix_least_fix spfStateLeast_dom spfStateLeast_ran)
+  then have f3:" spfStateLeast {c1} {c2} \<sqsubseteq> fixg (spfStateLeast {c1} {c2})(\<Lambda> f. f)"
+    by (smt fun_below_iff spfLeast_bottom spfStateLeast_def spfStateLeast_dom spfStateLeast_ran spfdom_eq spfran_eq)
+  show "fixg (spfStateLeast {c1} {c2}) (\<Lambda> f. f) = spfStateLeast {c1} {c2}"
+    using f2 f3 below_antisym by auto
+qed
+  
 section \<open>Lemmas for Composition\<close>
   (* this is only a part of the composition related lemmata, see SPF_Comp.thy *)
     
